Post crash interaction with knowledge of abstract history

src/high/post_crash_modality.v
@@ -1,3 +1,4 @@
+From iris.algebra Require Import auth.
 From self.base Require Import primitive_laws.
 From self.base Require post_crash_modality.
 From self.high Require Import dprop weakestpre.
@@ -6,9 +7,29 @@ Set Default Proof Using "Type".
 
 Notation base_post_crash := post_crash_modality.post_crash.
 
+Definition know_history_post_crash {Σ}
+            (hG : nvmG Σ) ℓ (hist : gmap time st) : iProp Σ :=
+  (∃ t state,
+    ⌜hist !! t = Some state⌝ ∗
+    know_full_encoded_history_loc ℓ ({[ 0 := state ]}) ∗
+    recovered {[ ℓ := MaxNat t ]}) ∨
+  (∀ t, ¬ (recovered {[ ℓ := MaxNat t ]})).
+
+(** This map is used to exchange [know_full_history_loc] valid prior to a crash
+into a version valid after the crash. *)
+Definition post_crash_map {Σ} (hh : gmap loc (gmap time st)) (hG hG' : nvmG Σ) : iProp Σ :=
+  (* Used to conclude that the locations owned are included in the heap in question. *)
+  (∀ ℓ hist, (know_full_encoded_history_loc (hG := hG) ℓ hist) -∗ ⌜hh !! ℓ = Some hist⌝) ∗
+  (* The map used to the the exchange. *)
+  [∗ map] ℓ ↦ hist ∈ hh,
+    (know_full_encoded_history_loc (hG := hG) ℓ hist) ∨ (know_history_post_crash hG' ℓ hist).
+
 Program Definition post_crash {Σ} (P : nvmG Σ → dProp Σ) `{hG : !nvmG Σ} : dProp Σ :=
-  MonPred
-    (λ TV, ∀ (hhG' : nvmHighG Σ), base_post_crash (λ hG', P (NvmG _ hG' hhG') (∅, ∅, ∅)))%I
+  MonPred (λ TV,
+    ∀ (hhG' : nvmHighG Σ) hh,
+      base_post_crash (λ hG',
+        (post_crash_map hh hG (NvmG _ hG' hhG')) -∗ P (NvmG _ hG' hhG') (∅, ∅, ∅)
+                                    ∗ (post_crash_map hh hG (NvmG _ hG' hhG'))))%I
     _.
 (* Next Obligation. solve_proper. Qed. *)
 
@@ -21,28 +42,71 @@ Section post_crash_prop.
   Implicit Types v : thread_val.
 
   (** Tiny shortcut for introducing the assumption for a [post_crash]. *)
-  Ltac iIntrosPostCrash := iIntros (hG').
+  Ltac iIntrosPostCrash := iIntros (hG' hh).
 
-  Lemma post_crash_intro Q:
-    (⊢ Q) →
-    (⊢ post_crash (λ _, Q)).
-  Proof.
-    iIntros (Hmono).
-    iIntrosPostCrash.
-    iFrame "∗".
-    iApply Hmono.
-  Qed.
+  (* Lemma post_crash_intro Q: *)
+  (*   (⊢ Q) → *)
+  (*   (⊢ post_crash (λ _, Q)). *)
+  (* Proof. *)
+  (*   iStartProof (iProp _). iIntros (TV'). *)
+  (*   iIntros (Hmono). *)
+  (*   iIntrosPostCrash. *)
+  (*   iFrame "∗". *)
+  (*   iApply Hmono. *)
+  (* Qed. *)
 
   Lemma post_crash_mono P Q:
     (∀ hG, P hG -∗ Q hG) →
     post_crash P -∗ post_crash Q.
   Proof.
-    iIntros (Hmono) "HP".
+    iStartProof (iProp _). iIntros (Hmono TV') "HP".
     iIntrosPostCrash.
     iDestruct ("HP" $! hG') as "P".
-    by iApply Hmono.
+    iApply (post_crash_modality.post_crash_mono with "P").
+    iIntros (hG2).
+    iIntros "P M".
+    iDestruct ("P" with "M") as "[P $]".
+    iDestruct (Hmono with "P") as "H".
+    done.
   Qed.
 
-  
+  Lemma post_crash_know_full_history_loc `{Countable ST} ℓ (abs_hist : abs_history ST) :
+    ⎡know_full_history_loc ℓ abs_hist⎤ -∗
+    post_crash (λ hG',
+      (∃ (t : time) (state : ST),
+        ⌜abs_hist !! t = Some state⌝ ∗
+        ⎡recovered {[ ℓ := MaxNat t ]}⎤ ∗
+        ⎡know_full_history_loc ℓ {[ 0 := state ]}⎤) ∨
+      (∀ t, ⎡¬ (recovered {[ ℓ := MaxNat t ]})⎤)).
+  Proof.
+    iStartProof (iProp _). iIntros (TV') "HP".
+    iIntrosPostCrash.
+    iDestruct (post_crash_modality.post_crash_intro with "HP") as "HP".
+    post_crash_modality.iCrash.
+    iIntros "[in M]".
+    rewrite know_full_equiv.
+    iAssert (⌜hh !! _ = Some _⌝)%I as %HI.
+    { iApply ("in" with "HP"). }
+    iDestruct (big_sepM_lookup_acc with "M") as "[[H|H] reIns]"; first done.
+    { iDestruct (own_valid_2 with "HP H") as %V.
+      rewrite -auth_frag_op in V.
+      apply auth_frag_valid_1 in V.
+      rewrite singleton_op in V.
+      apply singleton_valid in V.
+      apply auth_auth_op_valid in V.
+      done. }
+    iDestruct ("reIns" with "[$HP]") as "$".
+    iFrame "in".
+    iDestruct "H" as "[H|H]"; [iLeft|iRight; iFrame].
+    iDestruct "H" as (t estate) "(%look & hist & rec)".
+    apply lookup_fmap_Some in look as [st [eq yo]].
+    iExists t, st.
+    iFrame "rec".
+    iSplit; first done.
+    rewrite know_full_equiv.
+    rewrite -eq.
+    rewrite map_fmap_singleton.
+    iFrame.
+  Qed.
 
 End post_crash_prop.
